Optativas/VFS/practicas/Clase5.Listas.fst
@@ -22,10 +22,7 @@ let rec sum_append (l1 l2 : list int)
   = match l1 with
     | [] -> ()
     | x::xs -> 
-      assert (sum_int l1 + sum_int l2 == x + sum_int xs + sum_int l2);
-      assert (sum_int (l1 @ l2) = sum_int(x::(xs @ l2)));
-      assert (sum_int (l1 @ l2) = x + sum_int (xs @ l2));
-      sum_append xs l2; // H.I (revisar, si se sacan los assert y se pone la HI funciona)
+      sum_append xs l2;
       ()
 
 
@@ -40,9 +37,6 @@ let rec len_append (l1 l2 : list int)
   = match l1 with
     | [] -> ()
     | x::xs -> 
-      assert (length l1 + length l2 == 1 + length xs + length l2);
-      assert (length (l1 @ l2) == length (x::(xs @ l2)));
-      assert (length (l1 @ l2) == 1 + length (xs @ l2));
       len_append xs l2;
       ()
 
@@ -60,14 +54,72 @@ let rec rev_int (xs : list int) : list int =
   | [] -> []
   | x::xs' -> snoc (rev_int xs') x
 
-let rev_append_int (xs ys : list int)
-  : Lemma (rev_int (xs @ ys) == rev_int ys @ rev_int xs)
-= admit()
+(* unit-tests *)
+let _ = assert (snoc (rev_int [1;2;3]) 4 == [3;2;1;4])
 
-let rev_rev (xs : list int)
-  : Lemma (rev_int (rev_int xs) == xs)
-= admit()
+// Lema para "rev_append_int"
+let rec snoc_append (l1 l2 : list int) (x : int)
+  : Lemma (snoc (l1 @ l2) x == l1 @ snoc l2 x)
+  = match l1 with
+  | [] -> ()
+  | _::xs -> snoc_append xs l2 x
 
-let rev_injective (xs ys : list int)
-  : Lemma (requires rev_int xs == rev_int ys) (ensures xs == ys)
-= admit()
+// rev_int "distribuye" sobre append
+let rec rev_append_int (l1 l2 : list int)
+  : Lemma (rev_int (l1 @ l2) == rev_int l2 @ rev_int l1)
+= match l1 with
+  | [] -> ()
+  | x::xs ->
+    rev_append_int xs l2;
+    snoc_append (rev_int l2) (rev_int xs) x;
+    ()
+
+// Doble reverse es identidad
+let rec rev_rev (l : list int)
+  : Lemma (rev_int (rev_int l) == l)
+  (*
+  l = x:xs
+
+  rev (rev l) = rev (rev x:xs);
+  rev (rev x:xs) = rev (snoc (rev xs) x);
+  rev (snoc (rev xs) x) = rev (rev xs @ [x]);
+  rev (rev xs @ [x]) = rev [x] @ rev (rev xs)
+  [x] @ xs = l
+
+  xs = [1, 2, 3] x = 4
+  rev (rev [1, 2, 3] @ [4]) = rev [3, 2, 1, 4] = [4, 1, 2, 3]
+  rev (rev [1, 2, 3]) @ rev [4] = rev [3, 2, 1] @ [4] = [1, 2, 3, 4]
+
+  Lema 1: snoc (rev l) x = rev l @ [x]
+  Lema 2: rev (rev l1 @ l2) = rev l2 @ rev (rev l1)
+  *)
+= match l with
+  | [] -> ()
+  | x::xs ->
+    assume (rev (rev l) = rev (rev xs @ [x]));
+    assume (rev (rev xs @ [x]) = rev [x] @ rev (rev xs));
+    assume (rev [x] = [x]);
+    rev_rev xs;
+    admit();
+    ()
+
+let rec rev_injective (l1 l2 : list int)
+  : Lemma (requires rev_int l1 == rev_int l2) (ensures l1 == l2)
+  (*
+  l1 = x:xs
+  l2 = y:ys
+
+  rev x:xs = rev y:ys => snoc (rev xs) x = snoc (rev ys) y => 
+  => rev xs @ [x] = rev ys @ [y] => H.I =>
+  => sx @ [x] = sx @ [y] => (assume sx = sy)
+  => [x] = [y] =>
+  *)
+= match l1 with
+  | [] -> ()
+  | x::xs -> 
+    match l2 with
+    | [] -> ()
+    | y::ys ->
+      assert (rev (x::xs) = rev (y::ys));
+      ()
+
